\subsection{1(b)}
Referring to Problem $1(a)$, determine $w_1, w_2$ and  $w_3$ such that
$$ \lx{^C}{\frac{\partial \pmb a_1}{\partial \theta}} = w_1 \pmb a_1 + w_2 \pmb a_2 + w_3 \pmb a_3$$

\textbf{\textit{sol.}}
We have,
\begin{align*}
    \lx{^C}{\frac{\partial \pmb a_1}{\partial \theta}}  &=
    \frac{\partial}{\partial \theta} [R_3(\phi)[1,:]R_1(\theta)] \times \lx{^C}{\pmb c}
    %==
    = R_3(\phi)[1,:] \frac{\partial R_1(\theta)}{\partial \theta} \times \lx{^C}{\pmb c}
    %===
    = R_3(\phi)[1,:] \frac{\partial R_1(\theta)}{\partial \theta} \times [R_3(\phi)R_1(\theta)]^{-1} \times \lx{^C}{\pmb a}\\
    %==
    &=R_3(\phi)[1,:] \frac{\partial R_1(\theta)}{\partial \theta} \times R_1^T(\theta) R_3^T(\phi)\times \lx{^C}{\pmb a}
    %==
    \qquad \left[ \because R_i^{-1} = R_i^T \right]\\
    %==
    &= \bm{\cos \phi & \sin \phi  & 0}
    \bm{
            0 & 0 & 0\\
            0 & -\sin \theta & \cos \theta\\
            0 & -\cos \theta & -\sin \theta
        }
    \bm{
            1 & 0 & 0\\
            0 & \cos \theta & -\sin \theta\\
            0 & \sin \theta & \cos \theta
    }
    \bm{
            \cos \phi & -\sin \phi  & 0\\
            \sin \phi & \cos \phi & 0\\
            0          & 0         & 1
        }
    \times \lx{^c}{\pmb a}\\
     %==
    &= \bm{\cos \phi & \sin \phi  & 0}
    \bm{
            0 & 0 & 0\\
            0 & 0 & 1\\
            0 & 1 & 0
        }
    \bm{
            \cos \phi & -\sin \phi  & 0\\
            \sin \phi & \cos \phi & 0\\
            0          & 0         & 1
        }
    \times \lx{^c}{\pmb a}
    %==
    = \bm{0 & 0 & \sin \phi} \times \lx{^c}{\pmb a}\\
    %==
    \text{Hence, }&\\
    & w_1 = w_2 = 0, \: w_3 = \sin \phi
\end{align*}
