\subsection{2(i) $\pmb \omega = (\dot{\pmb a} \times \dot{\pmb b}) / (\dot{\pmb a} . \pmb b)$}

Consider,
\begin{align*}
    \dot{\pmb a} \times \dot{\pmb b} &= \dot{\pmb a} \times (\pmb \omega \times \pmb b) = (\dot{\pmb a}.\pmb b)\pmb \omega - \underbrace{(\dot{\pmb a} . \pmb \omega)}_{=0} \pmb b
    %===
    \qquad
    \bm{\because& \pmb a \times (\pmb b \times \pmb c) = (\pmb a.\pmb c)\pmb b - (\pmb a.\pmb b)\pmb c\\
    \because& (\pmb \omega \times \pmb a) \times \pmb \omega = 0 }\\
    %===
    \implies \pmb \omega &= \frac{\dot{\pmb a} \times \dot{\pmb b}}{(\dot{\pmb a}.\pmb b)} &q.e.d
\end{align*}
